AP/AP/Defense/Edge/WF.lean
@@ -19,57 +19,41 @@ def cnd (e : Edge) (s : State) : Prop :=
 instance {e : Edge} {s} : Decidable # e.cnd s := by
   simp [Edge.cnd]; split <;> all_goals infer_instance
 
--- #check 0 #exit
-
-theorem wf_defense_of_down (H : e.dir = .down) : e.defense.WF := by
+theorem wf_defense_of_down (h : e.dir = .down) : e.defense.WF := by
   sorry
 
 -- #check 0 #exit
 
-theorem wf_defense : e.defense.WF := by
-  -- use e.validTr_defense
-  -- intro s hs h a ha d hd n
-  -- cases H : e.dir
-  -- ·
-  --   -- obtain ⟨h₁, h₂⟩ := e.flipV.wf_defense_of_down (by simp [H])
-  --   -- have H₁ : Fact # e.flipV.dir = .down; simp [H]
-  --   -- specialize @h₂ (flipV.fs s) _ _ (a.sym flipV) _ (d.sym flipV) _ n
-  --   -- · simp [Edge.defense] at h ⊢; exact h
-  --   -- simp at h₂ ⊢
-  --   -- have h₃ := congrArg (·.sym rot180) e.flipV.defense_flipV_of_up
-  --   -- simp at h₃
-  --   -- rw [←h₃] at h₂; clear h₃
-  --   -- sorry
-  --   sorry
-  -- ·
-  --   -- obtain ⟨h₁, h₂⟩ := e.rotRight.wf_defense_of_up (by simp [H])
-  --   -- have H₁ : Fact e.rotRight.hor; simp [H]
-  --   -- have h₃ := e.rotRight.defense_rotRight_of_hor
-  --   -- specialize @h₂ s _ _
-  --   sorry
-  -- ·
-  --   -- obtain ⟨h₁, h₂⟩ := e.rotRight.wf_defense_of_up (by simp [H])
-  --   -- have H₁ : Fact e.rotRight.hor; simp [H]
-  --   -- specialize @h₂ (rotRight.fs s) _ _ (a.sym rotRight) _ (d.sym rotRight) _ n
-  --   -- · simp [Edge.defense] at h ⊢; exact h
-  --   -- convert h₂ using 2
-  --   -- · symm
-  --   sorry
-  -- · apply wf_defense_of_down H |>.2 h
-  
-  cases h : e.dir
-  · have H : Fact # e.dir = .up; use h
-    have h₁ := congrArg (·.sym rot180) e.defense_flipV_of_up
-    simp at h₁
-    rw [←h₁]; clear h₁
-    have h₁ : e.flipV.defense.WF
-    · apply wf_defense_of_down; simp
-    sorry
-    
-  · sorry
-  · sorry
-  · exact wf_defense_of_down h
+theorem wf_defense_of_up (h : e.dir = .up) : e.defense.WF := by
+  have H : Fact # e.dir = .up; use h
+  have h₁ := congrArg (·.sym rot180) e.defense_flipV_of_up
+  simp at h₁
+  rw [←h₁]; clear h₁
+  have h₁ : e.flipV.defense.WF
+  · apply wf_defense_of_down; simp
+  infer_instance
 
--- #check 0 #exit
+theorem wf_defense : e.defense.WF := by
+  cases h : e.dir
+  · exact wf_defense_of_up h
+  · have h₁ : e.rotLeft.defense.WF
+    · apply wf_defense_of_down; simp [h]
+    
+    have h₂ : e.rotLeft.rotRight.defense = e.rotLeft.defense.sym rotRight
+    · have H : Fact # e.rotLeft.hor; simp [h]
+      exact defense_rotRight_of_hor
+    simp at h₂
+    rw [h₂]
+    simpa
+  · have h₁ : e.rotLeft.defense.WF
+    · apply wf_defense_of_up; simp [h]
+    
+    have h₂ : e.rotLeft.rotRight.defense = e.rotLeft.defense.sym rotRight
+    · have H : Fact # e.rotLeft.hor; simp [h]
+      exact defense_rotRight_of_hor
+    simp at h₂
+    rw [h₂]
+    simpa
+  · exact wf_defense_of_down h
 
 @[simp] instance : e.defense.WF := wf_defense
